proofs/isabelle/SpecRest/core/Smt.thy
@@ -1,15 +1,17 @@
 theory Smt
-  imports IR
+  imports IR "HOL.Rat"
 begin
 
 datatype (plugins only: code size) smt_sort =
     SortBool
   | SortInt
+  | SortReal
   | SortUninterp "String.literal"
 
 datatype (plugins only: code size) smt_val =
     SBool bool
   | SInt int
+  | SReal rat
   | SEnumElem "String.literal" "String.literal"
   | SEntityElem "String.literal" "String.literal"
   | SSet "smt_val list"
@@ -18,6 +20,7 @@ datatype (plugins only: code size) smt_val =
 datatype (plugins only: code size) smt_term =
     BLit bool
   | ILit int
+  | RLit rat
   | TVar "String.literal"
   | EnumElemConst "String.literal" "String.literal"
   | TNot "smt_term"
@@ -170,6 +173,7 @@ and smtEval_forall_rel ::
 where
   "smtEval m env (BLit b) = Some (SBool b)"
 | "smtEval m env (ILit n) = Some (SInt n)"
+| "smtEval m env (RLit r) = Some (SReal r)"
 | "smtEval m env (TVar x) =
      (case smt_env_lookup env x of
         Some v \<Rightarrow> Some v
@@ -199,32 +203,53 @@ where
       | _ \<Rightarrow> None)"
 | "smtEval m env (TEq l r) =
      (case (smtEval m env l, smtEval m env r) of
-        (Some a, Some b) \<Rightarrow> Some (SBool (a = b))
+        (Some (SInt a), Some (SReal b)) \<Rightarrow> Some (SBool (of_int a = b))
+      | (Some (SReal a), Some (SInt b)) \<Rightarrow> Some (SBool (a = of_int b))
+      | (Some a, Some b) \<Rightarrow> Some (SBool (a = b))
       | _ \<Rightarrow> None)"
 | "smtEval m env (TLt l r) =
      (case (smtEval m env l, smtEval m env r) of
         (Some (SInt a), Some (SInt b)) \<Rightarrow> Some (SBool (a < b))
+      | (Some (SReal a), Some (SReal b)) \<Rightarrow> Some (SBool (a < b))
+      | (Some (SInt a), Some (SReal b)) \<Rightarrow> Some (SBool (of_int a < b))
+      | (Some (SReal a), Some (SInt b)) \<Rightarrow> Some (SBool (a < of_int b))
       | _ \<Rightarrow> None)"
 | "smtEval m env (TNeg t) =
      (case smtEval m env t of
         Some (SInt n) \<Rightarrow> Some (SInt (- n))
+      | Some (SReal n) \<Rightarrow> Some (SReal (- n))
       | _             \<Rightarrow> None)"
 | "smtEval m env (TAdd l r) =
      (case (smtEval m env l, smtEval m env r) of
         (Some (SInt a), Some (SInt b)) \<Rightarrow> Some (SInt (a + b))
+      | (Some (SReal a), Some (SReal b)) \<Rightarrow> Some (SReal (a + b))
+      | (Some (SInt a), Some (SReal b)) \<Rightarrow> Some (SReal (of_int a + b))
+      | (Some (SReal a), Some (SInt b)) \<Rightarrow> Some (SReal (a + of_int b))
       | _ \<Rightarrow> None)"
 | "smtEval m env (TSub l r) =
      (case (smtEval m env l, smtEval m env r) of
         (Some (SInt a), Some (SInt b)) \<Rightarrow> Some (SInt (a - b))
+      | (Some (SReal a), Some (SReal b)) \<Rightarrow> Some (SReal (a - b))
+      | (Some (SInt a), Some (SReal b)) \<Rightarrow> Some (SReal (of_int a - b))
+      | (Some (SReal a), Some (SInt b)) \<Rightarrow> Some (SReal (a - of_int b))
       | _ \<Rightarrow> None)"
 | "smtEval m env (TMul l r) =
      (case (smtEval m env l, smtEval m env r) of
         (Some (SInt a), Some (SInt b)) \<Rightarrow> Some (SInt (a * b))
+      | (Some (SReal a), Some (SReal b)) \<Rightarrow> Some (SReal (a * b))
+      | (Some (SInt a), Some (SReal b)) \<Rightarrow> Some (SReal (of_int a * b))
+      | (Some (SReal a), Some (SInt b)) \<Rightarrow> Some (SReal (a * of_int b))
       | _ \<Rightarrow> None)"
 | "smtEval m env (TDiv l r) =
      (case (smtEval m env l, smtEval m env r) of
         (Some (SInt a), Some (SInt b)) \<Rightarrow>
           (if b = 0 then None else Some (SInt (a div b)))
+      | (Some (SReal a), Some (SReal b)) \<Rightarrow>
+          (if b = 0 then None else Some (SReal (a / b)))
+      | (Some (SInt a), Some (SReal b)) \<Rightarrow>
+          (if b = 0 then None else Some (SReal (of_int a / b)))
+      | (Some (SReal a), Some (SInt b)) \<Rightarrow>
+          (if b = 0 then None else Some (SReal (a / of_int b)))
       | _ \<Rightarrow> None)"
 | "smtEval m env (TInDom rel_name arg) =
      (case smtEval m env arg of
